Fix regression

src/Pyrosome/Tools/EGraph/TypeInference.v
@@ -4,20 +4,31 @@ Require Import Datatypes.String Lists.List.
 Import ListNotations.
 Open Scope string.
 Open Scope list.
-From Utils Require Import Utils EGraph.Defs Monad.
-From Pyrosome Require Import Theory.Core Elab.Elab Tools.Matches Lang.SimpleVSubst Lang.SimpleVSTLC Tools.EGraph.Defs
-  Tools.EGraph.Automation Tools.EGraph.Test.
+From Utils Require Import Utils EGraph.Defs Monad Lens.
+From Pyrosome Require Import Theory.Core Elab.Elab Tools.Matches Tools.EGraph.Defs
+  Tools.EGraph.Automation.
 Require Import Utils.EGraph.Semantics.
 Import PArith.
 Import Ascii.AsciiSyntax.
 Import StringInstantiation.
 Import StateMonad.
 Require Import Coq.Strings.String.
-Require Import Coq.Numbers.DecimalString.
-Require Import Coq.Init.Nat.
+Require Coq.Numbers.DecimalString.
+
+
+Notation named_list := (@named_list string).
+Notation named_map := (@named_map string).
+Notation term := (@term string).
+Notation ctx := (@ctx string).
+Notation sort := (@sort string).
+Notation subst := (@subst string).
+Notation rule := (@rule string).
+Notation lang := (@lang string).
+
+(* TODO: make all of this use something other than strings *)
 
 Definition nat_to_string (n : nat) : string :=
-  NilZero.string_of_uint (Nat.to_uint n).
+  DecimalString.NilZero.string_of_uint (Nat.to_uint n).
 
 Fixpoint Zip_two_lists (X: Type) (Y: Type) (l1: list X) (l2: list Y) : list (X * Y) :=
   match l1 with
@@ -42,6 +53,9 @@ Fixpoint map_indexed (X: Type) (Y: Type) (f : nat -> X -> Y) (L: list X) (start:
 
 (* ------BUILDING_TERMS_and_SORTS_WITH_HOLES---------*)
 Local Open Scope string_scope.
+
+
+(*
 Fixpoint insert_terms_into_context
       (list_of_subterms: list term) (explicit_args: list string) (context: ctx) (prefix: string) : list term :=
   match context with
@@ -52,46 +66,12 @@ Fixpoint insert_terms_into_context
     | Some t => (cons t (insert_terms_into_context list_of_subterms explicit_args rest_context prefix))
     end
   end.
-Fixpoint build_term_with_holes_given_prefix (L: lang) (prefix: string) (index: nat) (t: term): term :=
-  match t with
-  | var _ => t
-  | con name_of_rule list_of_subterms =>
-      match NamedList.named_list_lookup
-        (term_rule [] [] (scon "ty" []))
-        L name_of_rule with
-          | term_rule context explicit_args some_sort_idk =>
-              con name_of_rule
-                (insert_terms_into_context
-                  ((map_indexed (build_term_with_holes_given_prefix L (prefix ++ (nat_to_string index) ++ "_"))) list_of_subterms 0)
-                  explicit_args
-                  context
-                  (prefix ++ (nat_to_string index) ++ "_"))
-          (* The case below never runs *)
-          | _ => t
-      end
-  end.
-Definition build_term_with_holes (L: lang) (t: term) :=
-  build_term_with_holes_given_prefix L "" 0 t.
-Definition build_sort_with_holes_given_prefix (L: lang) (prefix: string) (index: nat) (s: sort): sort :=
-  match s with
-  | scon name_of_rule list_of_subterms =>
-      match NamedList.named_list_lookup
-        (sort_rule [] [])
-        L name_of_rule with
-          | sort_rule context explicit_args =>
-              scon name_of_rule
-                (insert_terms_into_context
-                  ((map_indexed (build_term_with_holes_given_prefix L (prefix ++ (nat_to_string index) ++ "_"))) list_of_subterms 0)
-                  explicit_args
-                  context
-                  (prefix ++ (nat_to_string index) ++ "_"))
-          | _ => s
-      end
-  end.
-Definition build_sort_with_holes (L: lang) (s: sort) :=
-  build_sort_with_holes_given_prefix L "" 0 s.
+ *)
 
 
+(*TODO: log dummy names as they are gensymmed.
+Use writer monad
+ *)
 Fixpoint get_dummy_names_from_term (t: term) : list string :=
   match t with
   | var _ => []
@@ -106,6 +86,9 @@ Definition get_dummy_names_from_sort (s: sort) : list string :=
   | scon _ subterms => fold_right (@app string) [] (map get_dummy_names_from_term subterms)
   end.
 
+Definition get_dummy_names_from_ctx (c : ctx) :=
+  flat_map get_dummy_names_from_sort (map snd c).
+
 Fixpoint get_dummy_rules (dummy_names: list string) : lang :=
   match dummy_names with
   | nil => nil
@@ -115,89 +98,141 @@ Definition get_dummy_context (dummy_names: list string): ctx :=
   map (fun name => (name, scon "ty" [])) dummy_names.
 (* ----------------------------------------*)
 
-Local Open Scope list_scope.
-Fixpoint build_ctx_with_holes (L: lang) (context: ctx) :=
-  (* takes a pre-elaboration context and a language it type-checks in.
+
+(* Newtype for clear typeclass inference*)
+Record ident := { get_ident : string }.
+
+Definition log {M L} `{StateMonad (list L) M} (new_log : list L) : M unit :=
+  @!let log <- get_state in
+    (set_state (new_log++log)%list).
+
+(*TODO: Move? multiple variants exist *)
+Definition gensym {M} `{StateMonad ident M} `{StateMonad (list (string * rule)) M}
+  : M string :=
+  @!let s <- get_state in
+    let _ <- log (get_dummy_rules [s.(get_ident)]) in
+    let _ <- set_state (Build_ident (string_succ s.(get_ident))) in
+    ret s.(get_ident).
+
+(*
+Definition gen_dummy_rules {M} `{StateMonad (list ident) M}
+  : M _ :=
+  @!let s <- get_state in
+    ret (get_dummy_rules (map get_ident s)). *)
+
+(*Parameterized by M for later convenience*)
+Section __.
+  Context {M} `{StateMonad ident M}
+  `{StateMonad (list (string * rule)) M}.
+
+  Fixpoint insert_arg_holes (s : list term) (c_names e_args : list string) 
+    : M (list term) :=
+    match c_names, e_args, s with
+    | [], _, _ => Mret []
+    | x::c_names', [], [] =>
+        @! let s' <- insert_arg_holes [] c_names' [] in
+          let  x_sym <- gensym in
+          ret (con x_sym [] :: s')
+    | x::c_names', y::e_args', e::s' =>
+        if eqb x y then
+          @! let s'' <- insert_arg_holes s' c_names' e_args' in
+            ret (e :: s'')
+        else 
+          @! let s'' <- insert_arg_holes s c_names' e_args in
+            let x_sym <- gensym in
+            ret (con x_sym [] :: s'')
+    | _, _, _ => Mret default
+    end.
+  
+  Fixpoint build_term_with_holes (t: term)
+    : M term :=
+    match t with
+    | var _ => Mret t
+    | con name_of_rule s =>
+        @! let l <- get_state in
+        match NamedList.named_list_lookup_err l name_of_rule with
+        | Some (term_rule context explicit_args _) =>
+            @! let s' <- list_Mmap build_term_with_holes s in
+              let s_holes <- insert_arg_holes s (map fst context) explicit_args in
+              ret con name_of_rule s_holes
+        (* The case below never runs *)
+        | _ => Mret default
+        end
+    end.
+
+  Definition build_sort_with_holes (s: sort)
+    : M sort :=
+    match s with
+    | scon name_of_rule s =>
+        @! let l <- get_state in
+        match NamedList.named_list_lookup_err l name_of_rule with
+        | Some (sort_rule context explicit_args) =>
+            @! let s' <- list_Mmap build_term_with_holes s in
+              let s_holes <- insert_arg_holes s (map fst context) explicit_args in
+              ret scon name_of_rule s_holes
+        (* The case below never runs *)
+        | _ => Mret default
+        end
+    end.
+
+  Local Open Scope list_scope.
+  Fixpoint build_ctx_with_holes (context: ctx)
+    : M _ :=
+    (* takes a pre-elaboration context and a language it type-checks in.
     outputs a context with holes and an extended language with the dummy rule and the additional context rules *)
-  match context with
-  | nil => (L, nil)
-  | (name_n, s) :: rest =>
-    let (L', elab_rest) := (build_ctx_with_holes L rest) in
-    let sort_with_no_variables := sort_var_to_con s in
-    let sort_with_holes := (build_sort_with_holes_given_prefix L' name_n 0 sort_with_no_variables) in
-    (
-      ((get_dummy_rules (get_dummy_names_from_sort sort_with_holes)) ++ [(name_n, term_rule [] [] sort_with_holes)] ++ L'),
-      (name_n , sort_with_holes) :: elab_rest
-    )
-  end.
+    match context with
+    | nil => Mret nil
+    | (name_n, s) :: context =>
+        @!let elab_context <- build_ctx_with_holes context in
+          let s_with_no_variables := sort_var_to_con s in
+          let s_holes <- build_sort_with_holes s_with_no_variables in
+          let _ <- log [(name_n, term_rule [] [] s_holes)] in
+          ret ((name_n , s_holes) :: elab_context)
+    end.
+  
+End __.
 
-
-
-(* Injection rules  *)
-Fixpoint equalize_terms (L1: list string) (L2: list string) : list (clause string string) :=
-  match L1, L2 with
-  | _, nil => nil
-  | nil, _ => nil
-  | head_1 :: rest_1, head_2 :: rest_2 =>
-    (eq_clause head_1 head_2) :: equalize_terms rest_1 rest_2
-  end.
 Local Open Scope string_scope.
-Definition injection_rule_from_name_and_rule (name: string) (r: rule) : sequent string string :=
-  match r with
-  | term_rule context _ _ =>
-        let arguments1 := (map (fun x => (fst x) ++ "1") context) in
-        let arguments2 := (map (fun x => (fst x) ++ "2") context) in
-                {|
-              seq_assumptions :=
-              [atom_clause
-                    {| atom_fn := name ; atom_args := arguments1; atom_ret := "x0" |};
-                  atom_clause
-                    {| atom_fn := name ; atom_args := arguments2; atom_ret := "x0" |}];
-              seq_conclusions := equalize_terms arguments1 arguments2
-            |}
-  | sort_rule context _ =>
-        let arguments1 := (map (fun x => (fst x) ++ "1") context) in
-        let arguments2 := (map (fun x => (fst x) ++ "2") context) in
-                {|
-              seq_assumptions :=
-              [atom_clause
-                    {| atom_fn := name ; atom_args := arguments1; atom_ret := "x0" |};
-                  atom_clause
-                    {| atom_fn := name ; atom_args := arguments2; atom_ret := "x0" |}];
-              seq_conclusions := equalize_terms arguments1 arguments2
-            |}
-  (* Case below should never run, but if it runs we return a trivial rule *)
-  | _ => {|
-              seq_assumptions :=
-              [atom_clause
-                    {| atom_fn := name ; atom_args := ["X"]; atom_ret := "x" |};
-                  atom_clause
-                    {| atom_fn := name ; atom_args := ["X"]; atom_ret := "x" |}];
-              seq_conclusions := equalize_terms ["X"] ["X"]
-            |}
+(* Injection rules *)
+Fixpoint equalize_terms (args inj_args : list string) : list (clause string string) :=
+  match args with
+  | [] => []
+  | arg_name::args =>
+      if inb arg_name inj_args then (eq_clause (arg_name++"1") (arg_name++"2")) :: equalize_terms args inj_args
+      else equalize_terms args inj_args
   end.
-Definition build_injection_rule (L: lang) (name: string): sequent string string :=
+
+(* Assumes r is a term rule or sort rule *)
+Definition injection_rule_from_name_and_rule (name: string) inj_args (r: rule) : sequent string string :=
+  (*TODO: fresh name for atom_ret*)
+  let ret_name := name ++" cong_ret" in
+  let context := get_ctx r in
+  let args := map fst context in
+  let arguments1 := (map (fun x => (fst x) ++ "1") context) in
+  let arguments2 := (map (fun x => (fst x) ++ "2") context) in
+  {|
+    seq_assumptions :=
+      [atom_clause (Build_atom name arguments1 ret_name);
+       atom_clause (Build_atom name arguments2 ret_name)];
+    seq_conclusions := equalize_terms args inj_args
+  |}.
+
+Definition build_injection_rule (L: lang) (schema: string * list string): sequent string string :=
+  let (name, inj_args) := schema in
   match Find_x name L with
   | Some r =>
-    injection_rule_from_name_and_rule name r
-  | None =>
-          {|
-              seq_assumptions :=
-              [atom_clause
-                    {| atom_fn := name ; atom_args := ["X"]; atom_ret := "x" |};
-                  atom_clause
-                    {| atom_fn := name ; atom_args := ["X"]; atom_ret := "x" |}];
-              seq_conclusions := equalize_terms ["X"] ["X"]
-            |}
+    injection_rule_from_name_and_rule name inj_args r
+  | None => Build_sequent _ _ default default
   end.
-Definition build_injection_rules (names: list string) (L: lang): list (sequent string string) :=
-  map (build_injection_rule L) names.
+Definition build_injection_rules (schemas: list (string * list string)) (L: lang): list (sequent string string) :=
+  map (build_injection_rule L) schemas.
 (* ----------------------------- *)
 
 Local Open Scope char_scope.
 Definition weight (a: atom string string) : option positive :=
 match a with
 | Build_atom (String "?" _) [] _ => None
+| Build_atom "@sort_of"%string _ _ => None
 | _ => Some (1 %positive)
 end.
 Local Open Scope string_scope.
@@ -211,6 +246,10 @@ Fixpoint con_to_var (context: ctx) (t: term) : term :=
       if (inb name (map fst context)) then (var name) else t
   | con name subterms => con name (map (con_to_var context) subterms)
   | _ => t
+  end.
+Definition con_to_var_sort (context: ctx) (t: sort) : sort :=
+  match t with
+  | scon name subterms => scon name (map (con_to_var context) subterms)
   end.
 Definition result_to_term (result: Result.result term) : term :=
   match result with
@@ -227,86 +266,262 @@ Definition term_to_sort (t: term) : sort :=
   | var x => scon x []
   | con n s => scon n s
   end.
-Definition state_operation (L: lang) (inj_rules: list string) :=
+
+Definition const_rules (l: lang) :=
+  (map (uncurry (rule_to_log_rule string_trie_map _
+                   string_succ sort_of l (analysis_result:=unit) 1000))
+  (filter (fun '(n,r) => inclb (get_ctx r) []) l)).
+
+
+(* TODO: is this only running the injection rules???
+   Needs to at least also run all constant rules,
+   also equations.
+
+   TODO: rename
+ *)
+Definition state_operation (L: lang) (inj_rules: list (string * list string)) :=
   @saturate_until string String.eqb string_succ
     (default (A:= string))
     string
     string_trie_map
     string_ptree_map_plus string_trie_map string_ptree_map_plus
     string_list_trie_map (option positive) (weighted_depth_analysis weight) (@PosListMap.compat_intersect)
-    100
+    1000
     (
     @QueryOpt.build_rule_set string String.eqb string_succ (default (A:= string))
       string  string_trie_map string_ptree_map_plus string_trie_map
-      string_list_trie_map 100  (build_injection_rules inj_rules L)
+      string_list_trie_map 1000  (build_injection_rules inj_rules L
+                                    ++ const_rules L)
     )
-    (Mret false) 100
-    .
+    (Mret false) 1000.
+
+Definition state_operation_testing (L: lang) (inj_rules: list (string * list string)) f1 f2 :=
+  @saturate_until string String.eqb string_succ
+    (default (A:= string))
+    string
+    string_trie_map
+    string_ptree_map_plus string_trie_map string_ptree_map_plus
+    string_list_trie_map (option positive) (weighted_depth_analysis weight) (@PosListMap.compat_intersect)
+    f1
+    (
+    @QueryOpt.build_rule_set string String.eqb string_succ (default (A:= string))
+      string  string_trie_map string_ptree_map_plus string_trie_map
+      string_list_trie_map 1000 (build_injection_rules inj_rules L
+                                   ++ const_rules L)
+    )
+    (Mret false) f2.
 
 (* Breaking up egraph operations: *)
 
-(* Definition add_elab_term (L: lang) (t: term) (Id: string): state instance string :=  *)
+Record infer_state : Type :=
+  {
+    infer_fresh : ident;
+    infer_lang : list (string * rule);
+    egraph : instance;
+  }.
 
-(* INFERENCE: *)
-Definition infer_term (L: lang) (inj_rules: list string) (context: ctx) (t: term) (s: sort) :=
-  let Language_plus_rules := L ++ (ctx_to_rules context) in
+Instance infer_state_fresh : Lens infer_state ident :=
+  {
+    lens_get := infer_fresh;
+    lens_set s i := Build_infer_state i s.(infer_lang) s.(egraph);
+  }.
+Instance infer_state_infer_lang : Lens infer_state (list (string * rule)) :=
+  {
+    lens_get := infer_lang;
+    lens_set s l := Build_infer_state s.(infer_fresh) l s.(egraph);
+  }.
+Instance infer_state_egraph : Lens infer_state instance :=
+  {
+    lens_get := egraph;
+    lens_set s g := Build_infer_state s.(infer_fresh) s.(infer_lang) g;
+  }.
+
+(* assumes l contains the context rules *)
+(*TODO: always take in a sort id?*)
+Definition add_elab_term_to_egraph (t: term) (sort_id: string)
+  : state infer_state string :=
   let term_with_no_variables := (var_to_con t) in
-  let term_with_holes := build_term_with_holes Language_plus_rules term_with_no_variables in
-  let new_context := context ++ get_dummy_context (get_dummy_names_from_term (term_with_holes)) in
-  let dummy_rules := get_dummy_rules (get_dummy_names_from_term (term_with_holes)) in
-  let '(str, inst2) := add_open_term weight (Language_plus_rules ++ dummy_rules) true [] term_with_holes empty_egraph in
-  let '(id_sort, inst3) := add_open_sort weight (Language_plus_rules ++ dummy_rules) true [] (sort_var_to_con s) inst2 in
-  let '(id_original_sort, inst4) := @hash_entry string String.eqb string_succ string string_trie_map string_trie_map string_list_trie_map
-                                 _ (weighted_depth_analysis weight) sort_of [str] inst3 in
-  let '(_, inst5) := @union string String.eqb (default (A:= string)) string string_trie_map string_trie_map string_list_trie_map
-                     _ (weighted_depth_analysis weight) id_sort id_original_sort inst4 in
+  @!let term_with_holes <- build_term_with_holes term_with_no_variables in
+    let l <- get_state in
+    let t_id <- state_embed (add_open_term weight l true [] term_with_holes) in
+    let _ <- state_embed (update_entry (Build_atom sort_of [t_id] sort_id)) in
+    ret t_id.
 
-  let '(_, inst6) := (state_operation L inj_rules) inst5 in
-  con_to_var new_context (result_to_term (extract_weighted inst6 1000 str)).
+Definition infer_add_open_sort s :=
+  @!let l <- get_state in
+    (state_embed (add_open_sort weight l true [] s)).
 
-Definition infer_sort (L: lang) (inj_rules: list string) (context: ctx) (s: sort) : sort :=
-  let Language_plus_rules := L ++ (ctx_to_rules context) in
+(* assumes l contains the context rules *)
+Definition add_elab_sort_to_egraph (s:sort)
+  : state infer_state _ :=
   let sort_with_no_variables := (sort_var_to_con s) in
-  let sort_with_holes := build_sort_with_holes Language_plus_rules sort_with_no_variables in
-  let dummy_rules := get_dummy_rules (get_dummy_names_from_sort (sort_with_holes)) in
-  let '(str, inst2) := add_open_sort weight (Language_plus_rules ++ dummy_rules) true [] sort_with_holes empty_egraph in
+  @!let sort_with_holes <- build_sort_with_holes sort_with_no_variables in
+    (infer_add_open_sort sort_with_holes).
 
-  let '(_, inst3) := (state_operation L inj_rules) inst2 in
-  term_to_sort(result_to_term (extract_weighted inst3 1000 str)).
+Definition add_ctx_with_holes_to_egraph (context: ctx)
+  : state infer_state _ :=
+  (* takes a context holes, a language it type checks in.
+      adds the sorts in the context to the egraph.
+      Note: Mmap is in the wrong direction,
+      so it might not be sound to fuse this
+      with building the context with holes
+   *)
+  list_Mmap (fun '(n, s) => Mbind (fun str => Mret (n, str))
+                              (infer_add_open_sort s))
+    context.
+    
+(* INFERENCE: *)
+(*
+Definition infer_term (L: lang) inj_rules (context: ctx) (t: term) (s: sort) :=
+  let Language_plus_rules := L ++ (ctx_to_rules context) in
+  (*TODO: what is this and why did I use it? 
+  let new_context := context ++ get_dummy_context (get_dummy_names_from_term (term_with_holes)) in
+   *)
+  (*TODO: check that add_sort doesn't need dummy rules (it shouldn't)*)
+  let '(t_id, counter, graph) :=
+    (@! let {stateT string (state instance)} sort_id <- lift (add_open_sort weight Language_plus_rules true [] (sort_var_to_con s)) in
+       let {stateT string (state instance)} (t_id, dummy_rules) <-
+             add_elab_term_to_egraph Language_plus_rules t sort_id in
+      let _ <- lift (state_operation Language_plus_rules inj_rules) in
+      ret {stateT string (state instance)} t_id) "?" empty_egraph
+  in
+  con_to_var context (result_to_term (extract_weighted graph 1000 t_id)).
+*)
 
-Fixpoint infer_ctx (L: lang) (inj_rules: list string) (context: ctx) : ctx :=
+Variant egraph_rule_ids :=
+  | sort_rule_ids (c_ids : named_list string) (args : list string)
+  | term_rule_ids (c_ids : named_list string) (args : list string) (t_id : string)
+  | sort_eq_rule_ids (c_ids : named_list string) (t_id1 t_id2 : string)
+  | term_eq_rule_ids (c_ids : named_list string) (e_id1 e_id2 t_id : string).
+
+Definition decode_term context graph t_id :=
+  con_to_var context (result_to_term (extract_weighted graph 1000 t_id)).
+
+Definition decode_sort context graph t_id :=
+  term_to_sort (decode_term context graph t_id).
+
+Fixpoint decode_ctx graph ids :=
+  match ids with
+  | [] => []
+  | (x,x_id)::ids =>
+      let context := decode_ctx graph ids in
+      (x, decode_sort context graph x_id)::context
+  end.
+
+(*TODO: use state composed w/ writer for dummy rules?*)
+Definition infer_rule_egraph (l: lang) inj_rules r :=
+  let context := get_ctx r in
+  let comp : state infer_state _ :=
+    @!
+      let context_with_holes <- build_ctx_with_holes context in
+      let c_ids <- add_ctx_with_holes_to_egraph context_with_holes in
+      let res <- match r with
+                 | sort_rule _ args => @!ret sort_rule_ids c_ids args
+                 | term_rule _ args t => 
+                     @!let t_id <- add_elab_sort_to_egraph t in
+                       ret term_rule_ids c_ids args t_id
+                 | sort_eq_rule _ t1 t2 => 
+                     @!let t1_id <- add_elab_sort_to_egraph t1 in
+                       let t2_id <- add_elab_sort_to_egraph t2 in
+                       ret sort_eq_rule_ids c_ids t1_id t2_id
+                 | term_eq_rule _ e1 e2 t => 
+                     @!let t_id <- add_elab_sort_to_egraph t in
+                       let e1_id <- add_elab_term_to_egraph e1 t_id in
+                       let e2_id <- add_elab_term_to_egraph e2 t_id in
+                       ret (term_eq_rule_ids c_ids e1_id e2_id t_id)  
+                 end
+      in
+      let l <- get_state (S:= lang) in
+      let _ <- state_embed (state_operation l inj_rules) in
+      ret res
+          
+  in
+  comp (Build_infer_state (Build_ident "?") l empty_egraph).
+
+
+Definition infer_rule_egraph_testing_initial (l: lang) r :=
+  let context := get_ctx r in
+  let comp : state infer_state _ :=
+    @!
+      let context_with_holes <- build_ctx_with_holes context in
+      let c_ids <- add_ctx_with_holes_to_egraph context_with_holes in
+      let res <- match r with
+                 | sort_rule _ args => @!ret sort_rule_ids c_ids args
+                 | term_rule _ args t => 
+                     @!let t_id <- add_elab_sort_to_egraph t in
+                       ret term_rule_ids c_ids args t_id
+                 | sort_eq_rule _ t1 t2 => 
+                     @!let t1_id <- add_elab_sort_to_egraph t1 in
+                       let t2_id <- add_elab_sort_to_egraph t2 in
+                       ret sort_eq_rule_ids c_ids t1_id t2_id
+                 | term_eq_rule _ e1 e2 t => 
+                     @!let t_id <- add_elab_sort_to_egraph t in
+                       let e1_id <- add_elab_term_to_egraph e1 t_id in
+                       let e2_id <- add_elab_term_to_egraph e2 t_id in
+                       ret (term_eq_rule_ids c_ids e1_id e2_id t_id)  
+                 end
+      in
+      ret res
+                
+  in
+  comp (Build_infer_state (Build_ident "?") l empty_egraph).
+    
+Definition decode_rule ids graph :=
+  match ids with
+  | sort_rule_ids c_ids args =>
+      let c := decode_ctx graph c_ids in
+      sort_rule c args
+  | term_rule_ids c_ids args t_id =>
+      let c := decode_ctx graph c_ids in
+      let t := decode_sort c graph t_id in
+      term_rule c args t
+  | sort_eq_rule_ids c_ids t1_id t2_id => 
+      let c := decode_ctx graph c_ids in
+      let t1 := decode_sort c graph t1_id in
+      let t2 := decode_sort c graph t2_id in
+      sort_eq_rule c t1 t2
+  | term_eq_rule_ids c_ids e1_id e2_id t_id => 
+      let c := decode_ctx graph c_ids in
+      let t := decode_sort c graph t_id in
+      let e1 := decode_term c graph e1_id in
+      let e2 := decode_term c graph e2_id in
+      term_eq_rule c e1 e2 t
+  end.
+
+Definition infer_rule (l: lang) inj_rules r :=
+  let '(ids, s) := infer_rule_egraph l inj_rules r in
+  decode_rule ids s.(egraph).
+
+Fixpoint infer_lang_ext l_base l inj_rules :=
+  match l with
+  | [] => []
+  | (n,r)::l =>
+      (* inj_rules may include a superset of the rules of l, but that's ok *)
+      let l' := infer_lang_ext l_base l inj_rules in
+      let r' := infer_rule (l'++l_base) inj_rules r in
+      (n,r')::l'
+  end.
+
+(*
+Definition infer_sort (L: lang) inj_rules (context: ctx) (s: sort) : sort :=
+  let Language_plus_rules := L ++ (ctx_to_rules context) in
+  (*TODO: what is this and why did I use it? 
+  let new_context := context ++ get_dummy_context (get_dummy_names_from_term (term_with_holes)) in
+   *)
+  (*TODO: check that add_sort doesn't need dummy rules (it shouldn't)*)
+  let '(t_id, counter, graph) :=
+    (@! let {stateT string (state instance)} (t_id, dummy_rules) <-
+             add_elab_sort_to_egraph Language_plus_rules s in
+      let _ <- lift (state_operation Language_plus_rules inj_rules) in
+      ret {stateT string (state instance)} t_id) "?" empty_egraph
+  in
+  term_to_sort (con_to_var context (result_to_term (extract_weighted graph 1000 t_id))).
+
+Fixpoint infer_ctx (L: lang) inj_rules (context: ctx) : ctx :=
   match context with
   | nil => nil
   | (n, s) :: rest =>
     let elab_rest := (infer_ctx L inj_rules rest) in
       (n, (infer_sort L inj_rules elab_rest s)) :: elab_rest
   end.
-
-Definition add_ctx_with_holes_to_egraph (L: lang) (context: ctx): (state instance (named_list string)) :=
-  (* takes a context holes, a language it type checks in.
-      adds the sorts in the context to the egraph. *)
-  list_Mmap ( fun '(n, s) => Mbind (fun str => Mret (n, str)) (add_open_sort weight L true [] s) ) context.
-
-
-Definition infer_rule (L: lang) (inj_rules: list string) (r: rule) :=
-  match r with
-  | sort_rule c args => sort_rule (infer_ctx L inj_rules c) args
-  | term_rule c args t => let ec := infer_ctx L inj_rules c in
-                          let et := infer_sort L inj_rules ec t in
-                          term_rule ec args et
-  | sort_eq_rule c t1 t2 => let ec := infer_ctx L inj_rules c in
-                            let et1 := infer_sort L inj_rules ec t1 in
-                            let et2 := infer_sort L inj_rules ec t2 in
-                            sort_eq_rule ec et1 et2
-  | term_eq_rule c e1 e2 t => let ec := infer_ctx L inj_rules c in
-                              let et := infer_sort L inj_rules ec t in
-                              let ee1 := infer_term L inj_rules ec e1 et in
-                              let ee2 := infer_term L inj_rules ec e2 et in
-                              term_eq_rule ec ee1 ee2 et
-  end.
-
-Fixpoint infer_lang (L: lang) (inj_rules: list string) :=
-  match L with
-  | nil => nil
-  | (n, r) :: rest => (n, infer_rule rest inj_rules r) :: (infer_lang rest inj_rules)
-  end.
+*)
